src/3d/Binding.fst
@@ -862,8 +862,8 @@ let rec check_field_action (env:env) (f:field) (a:action)
         | Action_abort ->
           Action_abort, tunit
 
-        | Action_field_pos ->
-          Action_field_pos, tuint64
+        | Action_field_pos_64 ->
+          Action_field_pos_64, tuint64
 
         | Action_field_ptr ->
           Action_field_ptr, puint8
